theories/c_toy_lang/melocoton/examples.v
@@ -1,0 +1,84 @@
+From iris.proofmode Require Import coq_tactics reduction spec_patterns.
+From iris.proofmode Require Export tactics.
+From melocoton.c_toy_lang Require Import lang notation melocoton.proofmode.
+From iris.prelude Require Import options.
+Import uPred.
+
+
+(** Heap tactics *)
+Section examples.
+
+Context `{!heapGS Σ}.
+ 
+Fixpoint fib (n:nat) : nat := match n with
+  0 => 0
+| S n' => match n' with 
+      0 => 1
+    | S n'' => fib n' + fib n'' end end.
+
+Definition fib_prog name (x:expr) := (if: "x" < #2 then "x" else (call: (&name) with ("x" - #1))
+           + (call: (&name) with ("x" - #2) ))%E.
+Definition fib_func name : function := Fun [BNamed "x"] (fib_prog name "x").
+Definition exampleProgram name : gmap string function :=
+  insert "fib" (fib_func name) ∅.
+
+Definition exampleEnv name : prog_environ := {|
+  weakestpre.prog := exampleProgram name;
+  T := λ s v wp, match (s,v) with
+      ("fiba", [ #(LitInt z) ]) => wp (#(fib (Z.to_nat z)))
+    | _ => ⌜False⌝%I end
+|}.
+
+(* A simple recursive function *)
+
+Lemma fib_prog_correct (n:nat)
+  : ⊢ (WP (call: &"fib" with (Val #n)) @ exampleEnv "fib"; ⊤ {{ v, ⌜v = #(fib n)⌝ }}).
+Proof.
+  iStartProof.
+  wp_pure _.
+  rewrite lookup_insert.
+  iLöb as "IH" forall (n).
+  wp_pure _.
+  destruct (bool_decide _) eqn:Heq.
+  - wp_pure _. iModIntro. apply bool_decide_eq_true in Heq.
+    assert (n=0 \/ n=1) as [-> | ->] by lia; done.
+  - wp_pure _. apply bool_decide_eq_false in Heq. wp_bind (FunCall _ _).
+    wp_pure _. wp_apply wp_wand.
+    { assert ((n-1)%Z=(n-1)%nat) as -> by lia. wp_pure _; rewrite lookup_insert. iApply "IH". }
+    iIntros (v) "->". wp_bind (FunCall _ _). wp_pure _. wp_apply wp_wand.
+    { assert ((n-2)%Z=(n-2)%nat) as -> by lia.  wp_pure _; rewrite lookup_insert. iApply "IH". }
+    iIntros (v) "->". wp_pure _. iModIntro. iPureIntro. rewrite <- Nat2Z.inj_add.
+    repeat f_equal.
+    assert (n = S (S (n-2))) as -> by lia.
+    cbn. do 2 f_equal. lia.
+Qed.
+
+(* A call to an axiomatically specified function *)
+
+Lemma fiba_prog_correct (n:nat)
+  : ⊢ (WP (call: &"fib" with (Val #n)) @ exampleEnv "fiba"; ⊤ {{ v, ⌜v = #(fib n)⌝ }}).
+Proof.
+  iStartProof.
+  wp_pure _.
+  rewrite lookup_insert.
+  wp_pure _.
+  destruct (bool_decide _) eqn:Heq.
+  - wp_pure _. iModIntro. apply bool_decide_eq_true in Heq.
+    assert (n=0 \/ n=1) as [-> | ->] by lia; done.
+  - wp_pure _. apply bool_decide_eq_false in Heq. wp_bind (FunCall _ _).
+    wp_pure _.
+    assert ((n-1)%Z=(n-1)%nat) as -> by lia.
+    iApply (wp_extern' _ "fiba" [ #((n-1)%nat)] _ _); first by (iPureIntro; vm_compute).
+    do 3 iModIntro. cbn. rewrite Nat2Z.id.
+    wp_pure _.
+    assert ((n-2)%Z=(n-2)%nat) as -> by lia. wp_bind (FunCall _ _).
+    iApply (wp_extern' _ "fiba" [ #((n-2)%nat)] _ _); first by (iPureIntro; vm_compute).
+    do 3 iModIntro. cbn. rewrite Nat2Z.id.
+    wp_pures.
+    iModIntro. iPureIntro. rewrite <- Nat2Z.inj_add.
+    repeat f_equal.
+    assert (n = S (S (n-2))) as -> by lia.
+    cbn. do 2 f_equal. lia.
+Qed.
+
+End examples.
