theories/c_toy_lang/notation.v
@@ -57,7 +57,7 @@ Notation "'if:' e1 'then' e2 'else' e3" := (If e1%E e2%E e3%E)
 Notation "'while:' e1 'do' e2" := (While e1%E e2%E)
   (at level 200, e1, e2 at level 200) : expr_scope.
 
-Notation "'call' ff '(' e1 , .. , en ')'" := (FunCall ff (cons e1 .. (cons en nil) ..))
+Notation "'call:' ff 'with' '(' e1 , .. , en ')'" := (FunCall ff%E (cons e1%E .. (cons en%E nil) ..))
   (at level 200, ff, e1, en at level 200) : expr_scope.
 
 Notation "'let:' x := e1 'in' e2" := (Let x%binder e1%E e2%E)
